BRAL

BRAL/Basic.lean
@@ -1,1 +1,317 @@
-def hello := "world"
+-- Based on Okasaki's Binary Random Access List
+import Mathlib.Tactic
+namespace BRAL
+-- DEFINITIONS
+-- Type
+inductive Tree (α : Type) : Type
+  | Leaf : α → Tree α
+  | Node : ℕ → Tree α → Tree α → Tree α -- ℕ = Size of the tree
+deriving Repr
+
+abbrev RList (α : Type) := List (Tree α)
+
+
+-- Tree size
+def size {α : Type} : Tree α → ℕ
+  | Tree.Leaf _       => 1
+  | Tree.Node n _ _   => n
+
+-- This invariant is preserved throughout the program by "link"
+axiom size_n {α : Type} (n : ℕ) (t1 : Tree α) (t2 : Tree α) :
+  size (Tree.Node n t1 t2) = (size t1) + (size t2)
+
+
+-- Init: Empty list
+def empty {α : Type} : RList α := []
+def isEmpty {α : Type} : RList α → Bool
+  | []  => true
+  | _   => false
+
+
+-- Cons
+def link {α : Type} : Tree α → Tree α → Tree α :=
+  fun t1 t2 ↦ Tree.Node (size t1 + size t2) t1 t2
+
+def consTree {α : Type} : Tree α → RList α → RList α
+  | t, []       => [t]
+  | t, t' :: ts =>
+        if size t = size t' then
+          consTree (link t t') ts
+        else
+          t :: t' :: ts
+
+def cons {α : Type} (x : α) (ts : RList α) : RList α :=
+  consTree (Tree.Leaf x) ts
+
+
+-- Lookup using index (in O(log n))
+def lookupTree {α : Type} : ℕ → Tree α → Option α
+  | 0, Tree.Leaf x        => some x
+  | _, Tree.Leaf _        => none
+  | i, Tree.Node _ t1 t2  =>
+        if i < size t1 then
+          lookupTree i t1
+        else
+          lookupTree (i - size t1) t2
+
+def lookup {α : Type} : ℕ → RList α → Option α
+  | _, []       => none
+  | i, t :: ts  =>
+        if i < size t then
+          lookupTree i t
+        else
+          lookup (i - size t) ts
+
+
+-- Update in-place (in O(log n))
+def updateTree {α : Type} : ℕ → α → Tree α → Tree α
+  | 0, y, Tree.Leaf _       => Tree.Leaf y
+  | _, _, Tree.Leaf x       => Tree.Leaf x
+  | i, y, Tree.Node n t1 t2 =>
+        if i < size t1 then
+          Tree.Node n (updateTree i y t1) t2
+        else
+          Tree.Node n t1 (updateTree (i - size t1) y t2)
+
+def update {α : Type} : ℕ → α → RList α → RList α
+  | _, _, []      => []
+  | i, y, t :: ts =>
+        if i < size t then
+          (updateTree i y t) :: ts
+        else
+          t :: (update (i - size t) y ts)
+
+
+
+-- CONVERSION
+def treeToList {α : Type} : Tree α → List α
+  | Tree.Leaf x       => [x]
+  | Tree.Node _ t1 t2 => treeToList t1 ++ treeToList t2
+
+def toList {α : Type} : RList α → List α
+  | []        => []
+  | t :: ts   => treeToList t ++ toList ts
+
+def toRList {α : Type} : List α → RList α
+  | []        => []
+  | t :: ts   => cons t (toRList ts)
+
+
+
+-- TESTING
+#eval isEmpty (α := ℕ) empty
+def one := (cons 1 empty)
+def two := cons 2 one
+def three := cons 3 two
+def four := cons 4 three
+def five := cons 5 four
+def six := cons 6 five
+def seven := cons 7 six
+
+#eval one
+#eval two
+#eval three
+#eval four
+#eval five
+#eval six
+#eval seven
+
+#eval lookup 0 seven
+#eval lookup 1 seven
+#eval lookup 2 seven
+#eval lookup 3 seven
+#eval lookup 4 seven
+#eval lookup 5 seven
+#eval lookup 6 seven
+#eval lookup 7 seven
+
+#eval lookup 0 (update 0 99 seven)
+#eval lookup 1 (update 0 99 seven)
+#eval lookup 2 (update 0 99 seven)
+#eval lookup 3 (update 0 99 seven)
+#eval lookup 4 (update 0 99 seven)
+#eval lookup 5 (update 0 99 seven)
+#eval lookup 6 (update 0 99 seven)
+#eval lookup 7 (update 0 99 seven)
+
+#eval lookup 0 (update 6 99 seven)
+#eval lookup 1 (update 6 99 seven)
+#eval lookup 2 (update 6 99 seven)
+#eval lookup 3 (update 6 99 seven)
+#eval lookup 4 (update 6 99 seven)
+#eval lookup 5 (update 6 99 seven)
+#eval lookup 6 (update 6 99 seven)
+#eval lookup 7 (update 6 99 seven)
+
+#eval lookup 0 (update 7 99 seven)
+#eval lookup 1 (update 7 99 seven)
+#eval lookup 2 (update 7 99 seven)
+#eval lookup 3 (update 7 99 seven)
+#eval lookup 4 (update 7 99 seven)
+#eval lookup 5 (update 7 99 seven)
+#eval lookup 6 (update 7 99 seven)
+#eval lookup 7 (update 7 99 seven)
+
+
+#eval toRList (α := ℕ) []
+#eval toRList [1]
+#eval toRList [1, 2]
+#eval toRList [1, 2, 3]
+#eval toRList [1, 2, 3, 4, 5, 6, 7]
+
+#eval toList one
+#eval toList two
+#eval toList three
+#eval toList four
+#eval toList five
+#eval toList six
+#eval toList seven
+
+
+
+-- VERIFICATION
+
+-- Linking trees is equal to list concateℕion
+lemma link_toList {α : Type} (t1 : Tree α) (t2 : Tree α) :
+  treeToList (link t1 t2) = treeToList t1 ++ treeToList t2 :=
+  by
+    cases t1 <;> cases t2 <;> simp [link, treeToList]
+
+-- Correctness of consTree
+lemma consTree_toList {α : Type} (t : Tree α) (ts : RList α) :
+  toList (consTree t ts) = treeToList t ++ (toList ts) :=
+  by
+    induction ts generalizing t with
+      | nil           => simp [consTree, toList]
+      | cons t' ts ih =>
+          by_cases h : size t = size t'
+          {
+            simp [consTree, h, toList, ih, link_toList, List.append_assoc]
+          }
+          {
+            simp [consTree, h, toList]
+          }
+
+-- Main result: Our implementation is equal to a cons-list
+theorem cons_correct {α : Type} (x : α) (ts : RList α) :
+  toList (cons x ts) = x :: toList ts :=
+  by
+    simp [cons, consTree_toList, treeToList]
+
+
+
+
+-- helper-lemma for operations lookup/update
+lemma length_eq {α : Type} (t : Tree α) :
+  size t = (treeToList t).length :=
+  by
+    induction t with
+      | Leaf x               =>
+          simp [size, treeToList]
+      | Node n t1 t2 ihl ihr =>
+          simp [treeToList]
+          rw [←ihl, ←ihr]
+          apply size_n
+
+
+
+-- Correctness lookup inside a single tree
+lemma tree_lookup_correct {α : Type} (t : Tree α) (i : ℕ) :
+  lookupTree i t = (treeToList t)[i]? :=
+  by
+    induction t generalizing i with
+      | Leaf x                =>
+          cases i <;> simp [lookupTree, treeToList]
+      | Node n t1 t2 ihl ihr  =>
+          by_cases h : i < size t1
+          {
+            simp [lookupTree, h, treeToList, ihl]
+            rw [length_eq] at h
+            set l_list := (treeToList t1)
+            set r_list := (treeToList t2)
+            simp [List.getElem?_append_left, h]
+          }
+          {
+            simp [lookupTree, h, treeToList, ihr]
+            rw [length_eq] at h
+            rw [length_eq]
+            set l_list := (treeToList t1)
+            set r_list := (treeToList t2)
+            simp [List.getElem?_append, h]
+          }
+
+-- Correctness lookup:
+-- Proof of equality with List.getElem?
+theorem lookup_correct {α : Type} (l : RList α) (i : ℕ) :
+  lookup i l = (toList l)[i]? :=
+  by
+    induction l generalizing i with
+      | nil           =>
+          simp [lookup, toList]
+      | cons t ts ih  =>
+          by_cases h : i < size t
+          {
+            simp [lookup, h, toList, tree_lookup_correct]
+            rw [length_eq] at h
+            simp [List.getElem?_append_left, h]
+          }
+          {
+            simp [lookup, h, toList, ih]
+            rw [length_eq] at h
+            rw [length_eq]
+            simp [List.getElem?_append, h]
+          }
+
+
+
+-- Correctness update inside a single tree
+lemma tree_update_correct {α : Type} (t : Tree α) (i : ℕ) (y : α) :
+  treeToList (updateTree i y t) = List.set (treeToList t) i y :=
+  by
+    induction t generalizing i with
+      | Leaf x                =>
+          cases i <;> simp [updateTree, treeToList, List.set]
+      | Node n t1 t2 ihl ihr  =>
+          by_cases h : i < size t1
+          {
+            simp [updateTree, h, treeToList, ihl]
+            rw [length_eq] at h
+            set l_list := (treeToList t1)
+            set r_list := (treeToList t2)
+            simp [h]
+          }
+          {
+            simp [updateTree, h, treeToList, ihr]
+            rw [length_eq] at h
+            rw [length_eq]
+            set l_list := (treeToList t1)
+            set r_list := (treeToList t2)
+            simp [List.set_append, h]
+          }
+
+-- Correctness update:
+-- Proof of equality with List.set
+theorem update_correct {α : Type} (l : RList α) (i : ℕ) (y : α) :
+  toList (update i y l) = List.set (toList l) i y :=
+  by
+    induction l generalizing i with
+      | nil           =>
+          simp [update, toList]
+      | cons t ts ih  =>
+          by_cases h : i < size t
+          {
+            simp [update, h, toList, tree_update_correct]
+            rw [length_eq] at h
+            simp [h]
+          }
+          {
+            simp [update, h, toList, ih]
+            rw [length_eq] at h
+            rw [length_eq]
+            set l_head := (treeToList t)
+            set l_tail := (toList ts)
+            simp [List.set_append, h]
+          }
+
+
+end BRAL
