README.md
@@ -1,1 +1,3 @@
 # BRAL
+
+Proving correctness of an implementation of a binary random access list (based on Okazaki's BRAL) in Lean 4.
